added BPCP -> FOL SAT

fo_terms.v
@@ -7,11 +7,54 @@
 (*         CeCILL v2 FREE SOFTWARE LICENSE AGREEMENT          *)
 (**************************************************************)
 
-Require Import List Arith.
+Require Import List Arith Eqdep_dec Lia.
 
 Require Import acc_irr.
 
 Set Implicit Arguments.
+
+Ltac msplit n := 
+  match n with 
+    | 0    => idtac 
+    | S ?n => split; [ | msplit n ]
+   end.
+
+Section le_lt_pirr.
+
+  (** lt and lt are proof irrelevant *)
+
+  (* a dependent induction principle for le *)
+  
+  Scheme le_indd := Induction for le Sort Prop.
+
+  Theorem le_pirr x y (H1 H2 : x <= y) : H1 = H2.
+  Proof.
+    revert H2.
+    induction H1 as [ | m H1 IH ] using le_indd; intro H2.
+
+    change (le_n x) with (eq_rect _ (fun n' => x <= n') (le_n x) _ eq_refl).
+    generalize (eq_refl x).
+    pattern x at 2 4 6 10, H2. 
+    case H2; [intro E | intros m l E].
+    rewrite UIP_dec with (p1 := E) (p2 := eq_refl); auto.
+    apply eq_nat_dec.
+    contradiction (le_Sn_n m); subst; auto.
+    
+    change (le_S x m H1) with (eq_rect _ (fun n' => x <= n') (le_S x m H1) _ eq_refl).
+    generalize (eq_refl (S m)).
+    pattern (S m) at 1 3 4 6, H2.
+    case H2; [intro E | intros p H3 E].
+    contradiction (le_Sn_n m); subst; auto.
+    injection E; intro; subst.
+    rewrite (IH H3).
+    rewrite UIP_dec with (p1 := E) (p2 := eq_refl); auto.
+    apply eq_nat_dec.
+  Qed.
+
+  Fact lt_pirr x y (H1 H2 : x < y) : H1 = H2.
+  Proof. simpl; intros; apply le_pirr. Qed.
+
+End le_lt_pirr.
 
 (** First a small vector library *)
 
@@ -22,6 +65,24 @@ Section vec.
   Inductive vec : nat -> Type :=
     | vec_nil  : vec 0
     | vec_cons : forall n, X -> vec n -> vec (S n).
+
+  Definition vec_head n (v : vec (S n)) := match v with @vec_cons _ x _ => x end.
+  Definition vec_tail n (v : vec (S n)) := match v with @vec_cons _ _ w => w end.
+
+  Let vec_head_tail_type n : vec n -> Prop := 
+    match n with
+      | 0   => fun v => v = vec_nil
+      | S n => fun v => v = vec_cons (vec_head v) (vec_tail v)
+    end.
+
+  Let vec_head_tail_prop n v :  @vec_head_tail_type n v.
+  Proof. induction v; simpl; auto. Qed.
+
+  Fact vec_0_nil (v : vec 0) : v = vec_nil.
+  Proof. apply (vec_head_tail_prop v). Qed.
+
+  Fact vec_head_tail n (v : vec (S n)) : v = vec_cons (vec_head v) (vec_tail v).
+  Proof. apply (vec_head_tail_prop v). Qed.
 
   Fixpoint vec2list n (v : vec n) :=
     match v with
@@ -67,6 +128,11 @@ Section vec.
 End vec.
 
 Arguments vec_nil {X}.
+
+Tactic Notation "vec" "split" hyp(v) "with" ident(n) :=
+  rewrite (vec_head_tail v); generalize (vec_head v) (vec_tail v); clear v; intros n v.
+
+Tactic Notation "vec" "nil" hyp(v) := rewrite (vec_0_nil v).
 
 Section vec_map.
 
@@ -117,6 +183,100 @@ Fixpoint vec_sum n (v : vec nat n) :=
     | vec_nil      => 0
     | vec_cons x v => x+vec_sum v
   end.
+
+Section list_in_map.
+
+  Variable (X Y : Type).
+
+  Fixpoint list_in_map l : (forall x, @In X x l -> Y) -> list Y.
+  Proof.
+    refine (match l with
+      | nil  => fun _ => nil
+      | x::l => fun f => f x _ :: @list_in_map l _
+    end).
+    + left; auto.
+    + intros y Hy; apply (f y); right; auto.
+  Defined.
+
+  Theorem In_list_in_map l f x (Hx : In x l) : In (f x Hx) (list_in_map l f).
+  Proof.
+    revert f x Hx.
+    induction l as [ | x l IHl ]; intros f y Hy.
+    + destruct Hy.
+    + destruct Hy as [ -> | Hy ].
+      * left; auto.
+      * right.
+        apply (IHl (fun z Hz => f z (or_intror Hz))).
+  Qed.
+
+End list_in_map.
+
+Section list_dec.
+
+  Variable (X : Type) (P Q : X -> Prop) (H : forall x, { P x } + { Q x }).
+  
+  Theorem list_dec l : { x | In x l /\ P x } + { forall x, In x l -> Q x }.
+  Proof.
+    induction l as [ | x l IHl ].
+    + right; intros _ [].
+    + destruct (H x) as [ Hx | Hx ].
+      1: { left; exists x; simpl; auto. }
+      destruct IHl as [ (y & H1 & H2) | H1 ].
+      * left; exists y; split; auto; right; auto.
+      * right; intros ? [ -> | ? ]; auto.
+  Qed.
+
+End list_dec.
+
+Section finite.
+
+  Definition finite_t X := { lX | forall x : X, In x lX }.
+
+  Theorem fin_length n : { ll | forall l : list bool, length l < n <-> In l ll }.
+  Proof. 
+    induction n as [ | n (ll & Hll) ].
+    + exists nil; intros; split; try lia; intros [].
+    + exists (nil :: map (cons true) ll ++ map (cons false) ll).
+      intros [ | [] l ]; simpl.
+      * split; auto; lia.
+      * split. 
+        - right; apply in_or_app; left; apply in_map_iff.
+          exists l; split; auto; apply Hll; lia.
+        - intros [ H | H ]; try discriminate.
+          apply in_app_or in H; destruct H as [ H | H ];
+            apply in_map_iff in H; destruct H as (m & H1 & H2);
+            apply Hll in H2; inversion H1; subst; try lia.
+      * split.
+        - right; apply in_or_app; right; apply in_map_iff.
+          exists l; split; auto; apply Hll; lia.
+        - intros [ H | H ]; try discriminate.
+          apply in_app_or in H; destruct H as [ H | H ];
+            apply in_map_iff in H; destruct H as (m & H1 & H2);
+            apply Hll in H2; inversion H1; subst; try lia.
+  Qed.
+
+  Theorem finite_t_bool_list n : finite_t { l : list bool | length l < n }.
+  Proof.
+    destruct (fin_length n) as (ll & Hll).
+    set (f (l : list bool) (H : In l ll) := exist (fun l => length l < n) l (proj2 (Hll l) H)).
+    exists (list_in_map _ f).
+    intros (l & Hl).
+    generalize Hl; intros H.
+    apply Hll in Hl.
+    replace (exist _ l H) with (f l Hl).
+    + apply In_list_in_map.
+    + unfold f; f_equal; apply lt_pirr.
+  Qed.
+
+  Theorem finite_t_option X : finite_t X -> finite_t (option X).
+  Proof.
+    intros (lX & HX).
+    exists (None :: map Some lX).
+    intros [x|]; simpl; auto.
+    right; apply in_map_iff; exists x; auto.
+  Qed.
+
+End finite.
 
 (** Then first order terms with signature *)
 
@@ -400,6 +560,15 @@ Section fo_subst_comp.
 
 End fo_subst_comp.
 
+Definition env_lift K (phi : nat -> K) k n :=
+  match n with
+    | 0   => k
+    | S n => phi n
+  end.
+
+Arguments env_lift K phi k n /.
+Local Notation "phi ↑ k" := (env_lift phi k) (at level 0).
+
 Section fol.
 
   Variable (fol_sym : Set) (fol_sym_ar : fol_sym -> nat)
@@ -414,37 +583,46 @@ Section fol.
     | fol_bin   : fol_bop -> fol_form -> fol_form -> fol_form
     | fol_quant : fol_qop -> fol_form -> fol_form.
 
-  Definition fo_term_subst_lift (f : nat -> fo_term nat fol_sym_ar) n :=
+  Notation 𝕋 := (fo_term nat fol_sym_ar).
+  Notation 𝔽 := fol_form.
+
+  (* Notation ⟦ ⟧ ⟪ ⟫ φ ψ σ ρ ↑ ⦃ ⦄ ⇡*)
+
+  Definition fo_term_subst_lift (σ : nat -> 𝕋) n :=
     match n with 
       | 0   => in_var 0
-      | S n => fo_term_map S (fo_term_subst f (in_var n))
+      | S n => fo_term_map S (fo_term_subst σ (in_var n))
     end.
 
-  Arguments fo_term_subst_lift f n /.
+  Arguments fo_term_subst_lift σ n /.
 
-  Fixpoint fol_subst (f : nat -> fo_term nat fol_sym_ar) A :=
+  Local Notation "⇡ σ" := (fo_term_subst_lift σ) (at level 0).
+
+  Local Reserved Notation "t '⦃' σ '⦄'" (at level 0).
+
+  Fixpoint fol_subst σ A :=
     match A with
       | fol_false     => fol_false
-      | @fol_atom p v => fol_atom (vec_map (fo_term_subst f) v)
-      | fol_bin c A B => fol_bin c (fol_subst f A) (fol_subst f B)
-      | fol_quant q A => fol_quant q (fol_subst (fo_term_subst_lift f) A) 
-    end.
+      | @fol_atom p v => fol_atom (vec_map (fo_term_subst σ) v)
+      | fol_bin c A B => fol_bin c (A⦃σ⦄) (B⦃σ⦄)
+      | fol_quant q A => fol_quant q (A⦃⇡σ⦄) 
+    end
+  where "A ⦃ σ ⦄" := (fol_subst σ A).
 
-  Fact fol_subst_ext f g : (forall n, f n = g n) -> forall A, fol_subst f A = fol_subst g A.
+  Fact fol_subst_ext σ ρ : (forall n, σ n = ρ n) -> forall A, A⦃σ⦄ = A⦃ρ⦄.
   Proof.
-    intros Hfg A; revert A f g Hfg. 
+    intros Hfg A; revert A σ ρ Hfg. 
     induction A as [ | p v | c A IHA B IHB | q A IHA ]; intros f g Hfg; simpl; f_equal; auto.
     + apply vec_map_ext; intros; apply fo_term_subst_ext; intros; auto.
     + apply IHA. intros [ | n ]; simpl; rew fot; f_equal; auto.
   Qed.
 
-  (** This theorem is the important one that shows substitution do compose 
+  (** This theorem is the important one that shows substitutions do compose 
       hence De Bruijn notation are handled correctly by substitutions *)
 
-  Fact fol_subst_comp f g A : fol_subst f (fol_subst g A) 
-                            = fol_subst (fun n => fo_term_subst f (g n)) A.
+  Fact fol_subst_subst σ ρ A : (A⦃σ⦄)⦃ρ⦄ = A⦃fun n => fo_term_subst ρ (σ n)⦄.
   Proof.
-    revert f g; induction A as [ | p v | b A IHA B IHB | q A IHA ]; simpl; intros f g; auto.
+    revert σ ρ; induction A as [ | p v | b A IHA B IHB | q A IHA ]; simpl; intros f g; auto.
     + f_equal.
       rewrite vec_map_map.
       apply vec_map_ext.
@@ -466,45 +644,39 @@ Section fol.
     Variable (X : Type) (sem_sym  : forall s, vec X (fol_sym_ar s) -> X)
                         (sem_pred : forall s, vec X (fol_pred_ar s) -> Prop).
 
-    Implicit Type phi : nat -> X.
+    Implicit Type φ : nat -> X.
 
-    Definition fot_sem phi : fo_term nat fol_sym_ar -> X.
+    Definition fot_sem φ : 𝕋 -> X.
     Proof.
       apply fo_term_recursion.
-      + exact phi.
+      + exact φ.
       + intros s _ w; exact (sem_sym w).
     Defined.
 
-    Fact fot_sem_fix_0 phi n : fot_sem phi (in_var n) = phi n.
+    Local Notation "'⟦' t '⟧'" := (fun φ => @fot_sem φ t) (at level 0).
+
+    (* Notation ⟦ ⟧ ⟪ ⟫ φ ψ σ 𝕋 𝔽 *)
+
+    Fact fot_sem_fix_0 φ n : ⟦in_var n⟧ φ = φ n.
     Proof. apply fo_term_recursion_fix_0. Qed.
 
-    Fact fot_sem_fix_1 phi s v : fot_sem phi (in_fot s v) = sem_sym (vec_map (fot_sem phi) v).
+    Fact fot_sem_fix_1 φ s v : ⟦in_fot s v⟧ φ = sem_sym (vec_map (fun t => ⟦t⟧ φ) v).
     Proof. apply fo_term_recursion_fix_1. Qed.
 
     Hint Rewrite fot_sem_fix_0 fot_sem_fix_1 : fo_term_db.
 
-    Fact fot_sem_ext phi psy : (forall n, phi n = psy n)
-                            -> forall t, fot_sem phi t = fot_sem psy t.
+    Fact fot_sem_ext φ ψ : (forall n, φ n = ψ n) -> forall t, ⟦t⟧ φ = ⟦t⟧ ψ.
     Proof.
       induction t; rew fot; f_equal; auto.
       apply vec_map_ext; intros; auto.
     Qed.
 
-    Fact fot_sem_subst phi f t : fot_sem phi (fo_term_subst f t) 
-                               = fot_sem (fun n => fot_sem phi (f n)) t.
+    Fact fot_sem_subst φ σ t : ⟦fo_term_subst σ t⟧ φ = ⟦t⟧ (fun n => ⟦σ n⟧ φ).
     Proof.
       induction t; rew fot; f_equal; auto.
       rewrite vec_map_map.
       apply vec_map_ext; intros; auto.
     Qed.
-
-    Definition phi_lift phi x n :=
-      match n with
-        | 0   => x
-        | S n => phi n
-      end.
-
-    Arguments phi_lift phi x n /.
 
     Definition fol_bin_sem b :=
       match b with
@@ -515,35 +687,77 @@ Section fol.
 
     Arguments fol_bin_sem b /.
 
-    Definition quant_sem K q (P : K -> Prop) :=
+    Fact fol_bin_sem_dec b A B : { A } + { ~ A } -> { B } + { ~ B } 
+                              -> { fol_bin_sem b A B }
+                               + { ~ fol_bin_sem b A B }.
+    Proof.
+      revert b; intros [] HA HB; simpl; tauto.
+    Qed.
+
+    Definition fol_quant_sem K q (P : K -> Prop) :=
       match q with
         | fol_ex => ex P
         | fol_fa => forall x, P x 
       end.
 
-    Arguments quant_sem K q P /.
+    Arguments fol_quant_sem K q P /.
 
-    Let quant_sem_equiv K (P Q : K -> Prop) : 
+    Fact fol_quant_sem_equiv K (P Q : K -> Prop) : 
               (forall k, P k <-> Q k) 
-            -> forall q, quant_sem q P <-> quant_sem q Q.
+            -> forall q, fol_quant_sem q P <-> fol_quant_sem q Q.
     Proof.
       intros H []; simpl.
       + split; intros (k & ?); exists k; apply H; auto.
       + split; intros ? k; apply H; auto. 
     Qed.
 
-    Fixpoint fol_sem phi A : Prop :=
+    Fact fol_quant_sem_dec lX (HX : forall x : X, In x lX) q (P : X -> Prop) : 
+              (forall x, { P x } + { ~ P x }) -> { fol_quant_sem q P } + { ~ fol_quant_sem q P }.
+    Proof.
+      revert q; intros [] H; simpl.
+      + destruct list_dec with (1 := H) (l := lX)
+          as [ (x & H1 & H2) | H1 ].
+        * left; firstorder.
+        * right; intros (y & Hy).
+          apply (H1 y); auto.
+      + destruct list_dec with (P := fun x => ~ P x) (Q := P) (l := lX)
+          as [ (x & H1 & H2) | H1 ].
+        * firstorder.
+        * right; contradict H2; auto.
+        * left; intros x; apply H1; auto.
+    Qed.
+
+    (* Notation ⟦ ⟧ ⟪ ⟫ φ ψ σ ↑ *)
+
+    Local Reserved Notation "'⟪' f '⟫'" (at level 0).
+
+    Fixpoint fol_sem φ A : Prop :=
       match A with
         | fol_false     => False
-        | @fol_atom p v => sem_pred (vec_map (fot_sem phi) v)
-        | fol_bin b A B => fol_bin_sem b (fol_sem phi A) (fol_sem phi B) 
-        | fol_quant q A => quant_sem q (fun x => fol_sem (phi_lift phi x) A)
-      end.
+        | fol_atom v    => sem_pred (vec_map (fun t => ⟦t⟧ φ) v)
+        | fol_bin b A B => fol_bin_sem b (⟪A⟫ φ) (⟪B⟫ φ) 
+        | fol_quant q A => fol_quant_sem q (fun x => ⟪A⟫ (φ↑x))
+      end
+    where "⟪ A ⟫" := (fun φ => fol_sem φ A).
 
-    Fact fol_sem_ext phi psy : (forall n, phi n = psy n)
-                            -> forall A, fol_sem phi A <-> fol_sem psy A.
+    Definition fol_big_disj := fold_right (fol_bin fol_disj) fol_false.
+
+    Fact fol_sem_big_disj lf φ : ⟪ fol_big_disj lf ⟫ φ <-> exists f, In f lf /\ ⟪ f ⟫ φ.
     Proof.
-      intros H A; revert A phi psy H.
+      induction lf as [ | f lf IHlf ]; simpl.
+      + split; try tauto; intros ( ? & [] & _).
+      + rewrite IHlf.
+        split.
+        * intros [ H | (g & H1 & H2) ].
+          - exists f; auto.
+          - exists g; auto.
+        * intros (g & [ <- | Hg ] & ?); auto.
+          right; exists g; auto.
+    Qed.
+
+    Fact fol_sem_ext φ ψ : (forall n, φ n = ψ n) -> forall A, ⟪A⟫ φ <-> ⟪A⟫ ψ.
+    Proof.
+      intros H A; revert A φ ψ H.
       induction A as [ | p v | b A IHA B IHB | q A IHA ]; simpl; intros phi psy H; try tauto.
       + match goal with | |- sem_pred ?x <-> sem_pred ?y => replace x with y; try tauto end.
         apply vec_map_ext; intros; apply fot_sem_ext; auto.
@@ -555,17 +769,18 @@ Section fol.
            intros [ | n ]; simpl; auto.
     Qed.
 
+    (* Notation ⟦ ⟧ ⟪ ⟫ φ ψ σ ↑ ⦃ ⦄*)
+
     (** Semantics commutes with substitutions ... good *)
 
-    Theorem fol_sem_subst phi f A : fol_sem phi (fol_subst f A)
-                                <-> fol_sem (fun n => fot_sem phi (f n)) A.
+    Theorem fol_sem_subst φ σ A : ⟪ A⦃σ⦄ ⟫ φ <-> ⟪A⟫ (fun n => ⟦σ n⟧ φ).
     Proof.
-      revert phi f; induction A as [ | p v | b A IHA B IHB | q A IHA ]; simpl; intros phi f; try tauto.
+      revert φ σ; induction A as [ | p v | b A IHA B IHB | q A IHA ]; simpl; intros phi f; try tauto.
       + match goal with | |- sem_pred ?x <-> sem_pred ?y => replace x with y; try tauto end.
         rewrite vec_map_map; apply vec_map_ext.
         intros; rewrite fot_sem_subst; auto.
       + destruct b; rewrite (IHA phi f), (IHB phi f); tauto.
-      + apply quant_sem_equiv; intros x. 
+      + apply fol_quant_sem_equiv; intros x. 
         rewrite IHA; apply fol_sem_ext; intros [ | n ].
         - simpl; rew fot; simpl; auto.
         - unfold fo_term_subst_lift.
@@ -575,9 +790,387 @@ Section fol.
           intros; cbv; auto.
     Qed.
 
+    Section decidable.
+
+      (** For the semantics relation to be decidable over a finite domain,
+         it is necessary and SUFFICIENT that the sem_pred relation is decidable
+         or equivalently, each predicate is interpreted as a map: vec X _ -> bool *)
+
+      Variable (lX : list X) (HX : forall x : X, In x lX).
+      Variable (Hpred : forall s v, { @sem_pred s v } + { ~ sem_pred v }).
+
+      Theorem fol_sem_dec A φ : { ⟪A⟫ φ } + { ~ ⟪A⟫ φ }.
+      Proof.
+        revert φ.
+        induction A as [ | p v | b A IHA B IHB | q A IHA ]; intros phi.
+        + simpl; tauto.
+        + simpl; apply Hpred.
+        + simpl fol_sem; apply fol_bin_sem_dec; auto.
+        + simpl fol_sem; apply fol_quant_sem_dec with (1 := HX); auto.
+      Qed.
+
+    End decidable.
+
   End semantics.
 
+  Definition fo_form_fin_SAT (A : 𝔽) := 
+       exists X s_sym s_pred l φ, @fol_sem X s_sym s_pred φ A
+                              /\  forall x : X, In x l.
+
 End fol.
+
+Hint Rewrite fo_term_vars_fix_0 fo_term_vars_fix_1  
+             fo_term_subst_fix_0 fo_term_subst_fix_1
+             fot_sem_fix_0 fot_sem_fix_1 : fo_term_db.
+
+Section pcp_hand.
+
+  Variable (X : Type) (lc : list (list X * list X)).
+
+  Inductive pcp_hand : list X -> list X -> Prop :=
+    | in_pcph_0 : forall x y, In (x,y) lc -> pcp_hand x y
+    | in_pcph_1 : forall x y u l, In (x,y) lc -> pcp_hand u l -> pcp_hand (x++u) (y++l).
+
+  (** Any hand is either a card or of the for x++p/y++q where
+      x/y is a non-void card and p/q is a hand *)
+
+  Lemma pcp_hand_inv p q : 
+       pcp_hand p q -> In (p,q) lc 
+                    \/ exists x y p' q', In (x,y) lc /\ pcp_hand p' q' 
+                                      /\ p = x++p' /\ q = y++q' 
+                        /\  (x <> nil /\ y = nil  
+                          \/ x = nil /\ y <> nil
+                          \/ x <> nil /\ y <> nil ).
+  Proof.
+    induction 1 as [ x y H | x y p q H1 H2 IH2 ].
+    + left; auto. 
+    + destruct x as [ | a x ]; [ destruct y as [ | b y ] | ].
+      * simpl; auto.
+      * right; exists nil, (b::y), p, q; simpl; msplit 4; auto.
+        right; left; split; auto; discriminate.
+      * right; exists (a::x), y, p, q; simpl; msplit 4; auto.
+        destruct y.
+        - left; split; auto; discriminate.
+        - right; right; split; discriminate.
+  Qed.
+
+  Definition PCP := exists l, pcp_hand l l.
+
+End pcp_hand.
+
+Tactic Notation "solve" "ite" :=
+      match goal with _ : ?x < ?y |- context[if le_lt_dec ?y ?x then _ else _]
+        => let G := fresh in destruct (le_lt_dec y x) as [ G | _ ]; [ exfalso; lia | ]
+      end.
+
+Section bpcp.
+
+  Variable lc : list (list bool * list bool).
+
+  Inductive m_sym := fb : bool -> m_sym | fe | fs.
+
+  Definition a_sym s := 
+    match s with
+      | fb _ => 1
+      | _   => 0
+    end.
+
+  Inductive m_pred := p_P | p_lt | p_eq.
+
+  Definition a_pred (p : m_pred) := 2.
+
+  Arguments a_sym s /.
+  Arguments a_pred p /.
+
+  Notation term := (fo_term nat a_sym).
+
+  Notation form := (fol_form a_sym a_pred).
+
+  Infix "⤑" := (fol_bin fol_imp) (at level 62, right associativity).
+  Infix "⟑" := (fol_bin fol_conj) (at level 60, right associativity).
+  Infix "⟇" := (fol_bin fol_disj) (at level 61, right associativity).
+  Notation "∀" := (fol_quant fol_fa).
+  Notation "∃" := (fol_quant fol_ex).
+
+  Infix "##" := (vec_cons) (at level 65, right associativity).
+  Notation "£" := (@in_var nat _ a_sym).
+  Notation ø := (vec_nil).
+ 
+  Notation e := (in_fot fe ø).
+  Notation "∗" := (in_fot fs ø).
+  Notation "⊥" := (fol_false a_sym a_pred).
+
+  Notation "¬" := (fun x => x ⤑ ⊥).
+  Notation 𝓟  := (fun x y => fol_atom a_pred p_P (x##y##ø)).
+  Notation "x ≡ y" := (fol_atom a_pred p_eq (x##y##ø)) (at level 59).
+  Notation "x ≺ y" := (fol_atom a_pred p_lt (x##y##ø)) (at level 59).
+
+  Notation f_ := (fun b x => @in_fot _ _ a_sym (fb b) (x##ø)).
+
+  Fixpoint lb_app (l : list bool) (t : term) : term :=
+    match l with 
+      | nil  => t
+      | b::l => f_ b (lb_app l t)
+    end.
+
+  Notation lb2term := (fun l => lb_app l e).
+
+  Definition phi_P := ∀ (∀ (𝓟  (£1) (£0) ⤑ ¬ (£1 ≡ ∗) ⟑ ¬ (£0 ≡ ∗))).
+
+  Definition lt_irrefl := ∀ (¬ (£0 ≺ £0)).
+  Definition lt_trans := ∀(∀(∀(£2 ≺ £1 ⤑ £1 ≺ £0 ⤑ £2 ≺ £0))).
+  Definition phi_lt := lt_irrefl ⟑ lt_trans.
+
+  Definition eq_neq (b : bool) := ∀(¬(f_ b (£0) ≡ e)).
+  Definition eq_inj (b : bool) := ∀(∀( ¬(f_ b (£1) ≡ ∗) ⤑ f_ b (£1) ≡ f_ b (£0) ⤑ £1 ≡ £0)).
+  Definition eq_real := ∀(∀(f_ true (£1) ≡ f_ false (£0) ⤑ f_ true (£1) ≡ ∗
+                                                         ⟑ f_ false (£0) ≡ ∗)).
+  Definition phi_eq := eq_neq true ⟑ eq_neq false 
+                     ⟑ eq_inj true ⟑ eq_inj false 
+                     ⟑ eq_real.
+
+  Definition lt_pair (u v x y : term) := (u ≺ x ⟑ v ≡ y) ⟇ (v ≺ y ⟑ u ≡ x) ⟇ (u ≺ x ⟑ v ≺ y).
+
+  Definition lt_simul (c : list bool * list bool) := 
+    let (s,t) := c 
+    in   (£1 ≡ lb2term s ⟑ £0 ≡ lb2term t)
+       ⟇ ∃(∃(𝓟 (£1) (£0) ⟑ £3 ≡ lb_app s (£1) ⟑ £2 ≡ lb_app t (£0) ⟑ lt_pair (£1) (£0) (£3) (£2) )).
+
+  Definition phi_simul := ∀(∀(𝓟 (£1) (£0) ⤑ fol_big_disj (map lt_simul lc))).
+
+  Definition phi_R := phi_P ⟑ phi_lt ⟑ phi_eq ⟑ phi_simul ⟑ ∃(𝓟 (£0) (£0)).
+
+  Section BPCP_fin_sat.
+
+    Variable (l : list bool) (Hl : pcp_hand lc l l). 
+
+    Let n := length l.
+
+    Let X := option { m : list bool | length m < S n }.
+    Let fin_X : finite_t X.
+    Proof. apply finite_t_option, finite_t_bool_list. Qed.
+
+    Let lX := proj1_sig fin_X.
+    Let HlX : forall p, In p lX.
+    Proof. apply (proj2_sig fin_X). Qed.
+
+    Let sem_sym : forall s, vec X (a_sym s) -> X.
+    Proof.
+      intros []; simpl.
+      + intros v.
+        case_eq (vec_head v).
+        * intros (m & Hm) H.
+          destruct (le_lt_dec n (length m)) as [ | H1 ].
+          - right.
+          - left; exists (b::m); apply lt_n_S, H1.
+        * right.
+      + left; exists nil; apply lt_0_Sn.
+      + right.
+    Defined.
+
+    Let sem_pred : forall p, vec X (a_pred p) -> Prop.
+    Proof.
+      intros []; simpl; intros v.
+      + destruct (vec_head v) as [ (s & Hs) | ].
+        2: exact False.
+        destruct (vec_head (vec_tail v)) as [ (t & Ht) | ].
+        2: exact False.
+        exact (pcp_hand lc s t).
+      + destruct (vec_head v) as [ (s & Hs) | ].
+        2: exact False.
+        destruct (vec_head (vec_tail v)) as [ (t & Ht) | ].
+        2: exact False.
+        exact (s <> t /\ exists u, u++s = t).
+      + exact (vec_head v = vec_head (vec_tail v)).
+    Defined.
+
+    Notation "⟦ t ⟧" := (fun φ => fot_sem sem_sym φ t).
+
+    Let fot_sem_lb_app lb t φ : 
+      match ⟦ t ⟧ φ with
+        | Some (exist _ m Hm) =>   
+          match le_lt_dec (S n) (length lb + length m) with
+            | left _  => ⟦ lb_app lb t ⟧ φ = None
+            | right _ => exists H, ⟦ lb_app lb t ⟧ φ = Some (exist _ (lb++m) H)
+          end
+        | None => ⟦ lb_app lb t ⟧ φ = None
+      end.
+    Proof.
+      induction lb as [ | x lb IH ]; simpl lb_app.
+      + destruct (⟦ t ⟧ φ) as [ (m & Hm) | ]; auto.
+        simpl plus; solve ite; simpl; exists Hm; auto.
+      + destruct (⟦ t ⟧ φ) as [ (m & Hm) | ]; auto.
+        2: { rew fot; simpl vec_map; rewrite IH; simpl; auto. }
+        simpl plus.
+        destruct (le_lt_dec (S n) (length lb + length m)) as [ H1 | H1 ].
+        * destruct (le_lt_dec (S n) (S (length lb+length m))) as [ H2 | H2 ].
+          2: exfalso; lia.
+          rew fot; simpl vec_map; rewrite IH; auto.
+        * destruct IH as (H2 & IH).
+          destruct (le_lt_dec (S n) (S (length lb+length m))) as [ H3 | H3 ].
+          - rew fot; simpl vec_map; rewrite IH; simpl.
+            destruct (le_lt_dec n (length (lb++m))) as [ | C ]; auto.
+            exfalso; rewrite app_length in C; lia.
+          - assert (length ((x::lb)++m) < S n) as H4.
+            { simpl; rewrite app_length; auto. }
+            exists H4; rew fot; simpl vec_map.
+            rewrite IH; simpl.
+            destruct (le_lt_dec n (length (lb++m))) as [ H5 | H5 ].
+            ++ exfalso; rewrite app_length in H5; lia.
+            ++ do 2 f_equal; apply lt_pirr.
+    Qed.
+
+    Let fot_sem_lb_app_Some lb t φ lt Ht (H : length (lb++lt) < S n) : 
+           ⟦ t ⟧ φ = Some (exist _ lt Ht) -> ⟦ lb_app lb t ⟧ φ = Some (exist _ (lb++lt) H).
+    Proof.
+      intros H1.
+      generalize (fot_sem_lb_app lb t φ); rew fot; simpl vec_map; rewrite H1.
+      rewrite <- app_length; solve ite.
+      intros (G & ->); do 2 f_equal; apply lt_pirr.
+    Qed.
+
+    Let fot_sem_lb_app_e lb φ (H : length lb < S n) : ⟦ lb_app lb e ⟧ φ = Some (exist _ lb H).
+    Proof.
+      revert H.
+      rewrite (app_nil_end lb); intros H.
+      rewrite <- app_nil_end at 1. 
+      apply fot_sem_lb_app_Some with (Ht := lt_0_Sn _).
+      rew fot; simpl; auto.
+    Qed.
+
+    Let φ : nat -> X := fun _ => None.
+
+    Notation "⟪ A ⟫" := (fol_sem sem_sym sem_pred φ A).
+
+    Let sem_phi_P : ⟪ phi_P ⟫.
+    Proof.
+      simpl; intros [ (x & Hx) | ] [ (y & Hy) | ]; simpl;
+      unfold env_lift; simpl; rew fot; unfold sem_sym in |- *; simpl; try tauto.
+      intros _; split; intros ?; discriminate.
+    Qed.
+
+    Let sem_phi_lt : ⟪ phi_lt ⟫.
+    Proof.
+      simpl; split.
+      + intros [ (x & Hx) | ]; simpl; auto.
+        intros ( [] & _ ); auto.
+      + intros [ (x & Hx) | ] [ (y & Hy) | ] [ (z & Hz) | ]; simpl; try tauto.
+        intros (H1 & H2) (H3 & H4); split.
+        * intros ->.
+          destruct H2 as (a & <-).
+          destruct H4 as (b & H4).
+          destruct b as [ | u b ].
+          - destruct a as [ | v a ].
+            ++ destruct H3; auto.
+            ++ apply f_equal with (f := @length _) in H4.
+               simpl in H4; rewrite app_length in H4; lia.
+          - apply f_equal with (f := @length _) in H4.
+            simpl in H4; do 2 rewrite app_length in H4; lia.
+        * clear H1 H3; revert H2 H4.
+          intros (a & <-) (b & <-).
+          exists (b++a); rewrite app_ass; auto.
+    Qed.
+
+    Let sem_phi_eq : ⟪ phi_eq ⟫.
+    Proof.
+      simpl; msplit 4.
+      1,2: intros [ (x & Hx) | ]; simpl; rew fot; unfold sem_sym; simpl; try discriminate;
+          destruct (le_lt_dec n (length x)) as [ | ]; try discriminate.
+      1,2: intros [ (x & Hx) | ] [ (y & Hy) | ]; simpl; rew fot; simpl; auto;
+          try destruct (le_lt_dec n (length x)) as [ | ]; try destruct (le_lt_dec n (length y)) as [ | ];
+          try discriminate; try tauto;
+          inversion 2; subst; repeat f_equal; apply lt_pirr.
+      intros [ (x & Hx) | ] [ (y & Hy) | ]; simpl; rew fot; simpl; auto;
+          try destruct (le_lt_dec n (length x)) as [ | ]; try destruct (le_lt_dec n (length y)) as [ | ];
+          try discriminate; try tauto.
+    Qed.
+
+    Opaque le_lt_dec.
+
+    Let list_app_head_not_nil K (u v : list K) : u <> nil -> v <> u++v.
+    Proof.
+      intros H; contradict H.
+      destruct u as [ | a u ]; auto; exfalso.
+      apply f_equal with (f := @length _) in H.
+      revert H; simpl; rewrite app_length; lia.
+    Qed.
+
+    Let sem_phi_simul : ⟪ phi_simul ⟫.
+    Proof.
+      simpl.
+      intros x y.
+      rewrite fol_sem_big_disj.
+      revert x y.
+      intros [ (x' & Hx) | ] [ (y' & Hy) | ]; simpl; rew fot; try tauto.
+      intros H.
+      apply pcp_hand_inv in H.
+      destruct H as [ H | (x & y & p & q & H1 & H2 & -> & -> & H) ].
+      + exists (lt_simul (x',y')); split.
+        * apply in_map_iff; exists (x',y'); auto.
+        * unfold lt_simul; simpl; left; split.
+          - rew fot.
+            rewrite fot_sem_lb_app_e with (H := Hx).
+            simpl; auto.
+          - rew fot.
+            rewrite fot_sem_lb_app_e with (H := Hy).
+            simpl; auto.
+      + exists (lt_simul (x,y)); split.
+        * apply in_map_iff; exists (x,y); split; auto.
+        * unfold lt_simul; right.          
+          exists (⟦lb_app p e⟧ φ), (⟦lb_app q e⟧ φ).
+          assert (length p < S n) as H5 by (rewrite app_length in Hx; lia).
+          assert (length q < S n) as H6 by (rewrite app_length in Hy; lia).
+          rewrite fot_sem_lb_app_e with (H := H5).
+          rewrite fot_sem_lb_app_e with (H := H6).
+          simpl; msplit 3; auto.
+          - rew fot.
+            rewrite fot_sem_lb_app_Some with (lt0 := p) (Ht := H5) (H := Hx).
+            ++ simpl; auto.
+            ++ rew fot; simpl; auto.
+          - rew fot.
+            rewrite fot_sem_lb_app_Some with (lt0 := q) (Ht := H6) (H := Hy).
+            ++ simpl; auto.
+            ++ rew fot; simpl; auto.
+          - destruct H as [ (G1 & G2) | [ (G1 & G2) | (G1 & G2) ] ].
+            ++ left; split.
+               ** split.
+                  -- revert G1; apply list_app_head_not_nil.
+                  -- exists x; auto.
+               ** rew fot; simpl; subst; do 2 f_equal; apply lt_pirr.
+            ++ right; left; split.
+               ** split.
+                  -- revert G2; apply list_app_head_not_nil.
+                  -- exists y; auto.
+               ** rew fot; simpl; subst; do 2 f_equal; apply lt_pirr.
+            ++ do 2 right; split.
+               ** split.
+                  -- revert G1; apply list_app_head_not_nil.
+                  -- exists x; auto.
+               ** split.
+                  -- revert G2; apply list_app_head_not_nil.
+                  -- exists y; auto.
+    Qed.
+
+    Let sem_phi_solvable :  ⟪ ∃(𝓟 (£0) (£0)) ⟫.
+    Proof.
+      simpl.
+      exists (Some (exist _ l (lt_n_Sn _))); simpl; auto.
+    Qed.
+
+    Theorem BPCP_sat : fo_form_fin_SAT phi_R.
+    Proof.
+      exists X, sem_sym, sem_pred, lX, φ; split; auto.
+      unfold phi_R; repeat (split; auto).
+    Qed.
+
+  End BPCP_fin_sat.
+
+  Check BPCP_sat.
+
+End bpcp.
+
+
+
 
 
     
